Lifetime logic: rename shared borrows to atomic (persistent) borrows

theories/lifetime/at_borrow.v
@@ -3,35 +3,35 @@ From iris.proofmode Require Import tactics.
 From lrust.lifetime Require Export lifetime.
 Set Default Proof Using "Type".
 
-(** Shared bors  *)
+(** Atomic persistent bors  *)
 (* TODO : update the TEX with the fact that we can choose the namespace. *)
-Definition shr_bor `{invG Σ, lftG Σ} κ N (P : iProp Σ) :=
+Definition at_bor `{invG Σ, lftG Σ} κ N (P : iProp Σ) :=
   (∃ i, &{κ,i}P ∗
     (⌜N ⊥ lftN⌝ ∗ inv N (idx_bor_own 1 i) ∨
      ⌜N = lftN⌝ ∗ inv N (∃ q, idx_bor_own q i)))%I.
-Notation "&shr{ κ , N } P" := (shr_bor κ N P)
-  (format "&shr{ κ , N }  P", at level 20, right associativity) : uPred_scope.
+Notation "&at{ κ , N } P" := (at_bor κ N P)
+  (format "&at{ κ , N }  P", at level 20, right associativity) : uPred_scope.
 
-Section shared_bors.
+Section atomic_bors.
   Context `{invG Σ, lftG Σ} (P : iProp Σ) (N : namespace).
 
-  Global Instance shr_bor_ne κ n : Proper (dist n ==> dist n) (shr_bor κ N).
+  Global Instance at_bor_ne κ n : Proper (dist n ==> dist n) (at_bor κ N).
   Proof. solve_proper. Qed.
-  Global Instance shr_bor_contractive κ : Contractive (shr_bor κ N).
+  Global Instance at_bor_contractive κ : Contractive (at_bor κ N).
   Proof. solve_contractive. Qed.
-  Global Instance shr_bor_proper : Proper ((⊣⊢) ==> (⊣⊢)) (shr_bor κ N).
+  Global Instance at_bor_proper : Proper ((⊣⊢) ==> (⊣⊢)) (at_bor κ N).
   Proof. solve_proper. Qed.
 
-  Lemma shr_bor_iff κ P' : ▷ □ (P ↔ P') -∗ &shr{κ, N} P -∗ &shr{κ, N} P'.
+  Lemma at_bor_iff κ P' : ▷ □ (P ↔ P') -∗ &at{κ, N} P -∗ &at{κ, N} P'.
   Proof.
     iIntros "HPP' H". iDestruct "H" as (i) "[HP ?]". iExists i. iFrame.
     iApply (idx_bor_iff with "HPP' HP").
   Qed.
 
-  Global Instance shr_bor_persistent : PersistentP (&shr{κ, N} P) := _.
+  Global Instance at_bor_persistent : PersistentP (&at{κ, N} P) := _.
 
   Lemma bor_share E κ :
-    ↑lftN ⊆ E → N ⊥ lftN → &{κ}P ={E}=∗ &shr{κ, N}P.
+    ↑lftN ⊆ E → N ⊥ lftN → &{κ}P ={E}=∗ &at{κ, N}P.
   Proof.
     iIntros (? HN) "HP". rewrite bor_unfold_idx. iDestruct "HP" as (i) "(#?&Hown)".
     iExists i. iFrame "#".
@@ -39,16 +39,16 @@ Section shared_bors.
   Qed.
 
   Lemma bor_share_lftN E κ :
-    ↑lftN ⊆ E → &{κ}P ={E}=∗ &shr{κ, lftN}P.
+    ↑lftN ⊆ E → &{κ}P ={E}=∗ &at{κ, lftN}P.
   Proof.
     iIntros (?) "HP". rewrite bor_unfold_idx. iDestruct "HP" as (i) "(#?&Hown)".
     iExists i. iFrame "#". subst.
     iRight. iSplitR. done. by iMod (inv_alloc with "[Hown]") as "$"; auto.
   Qed.
 
-  Lemma shr_bor_acc E κ :
+  Lemma at_bor_acc E κ :
     ↑lftN ⊆ E → ↑N ⊆ E →
-    lft_ctx -∗ &shr{κ,N}P ={E,E∖↑N∖↑lftN}=∗ ▷P ∗ (▷P ={E∖↑N∖↑lftN,E}=∗ True) ∨
+    lft_ctx -∗ &at{κ,N}P ={E,E∖↑N∖↑lftN}=∗ ▷P ∗ (▷P ={E∖↑N∖↑lftN,E}=∗ True) ∨
                [†κ] ∗ |={E∖↑N∖↑lftN,E}=> True.
   Proof.
     iIntros (??) "#LFT #HP". iDestruct "HP" as (i) "#[Hidx [[% Hinv]|[% Hinv]]]".
@@ -63,45 +63,45 @@ Section shared_bors.
       + iRight. iFrame. iIntros "!>". by iMod "Hclose".
   Qed.
 
-  Lemma shr_bor_acc_tok E q κ :
+  Lemma at_bor_acc_tok E q κ :
     ↑lftN ⊆ E → ↑N ⊆ E →
-    lft_ctx -∗ &shr{κ,N}P -∗ q.[κ] ={E,E∖↑N}=∗ ▷P ∗ (▷P ={E∖↑N,E}=∗ q.[κ]).
+    lft_ctx -∗ &at{κ,N}P -∗ q.[κ] ={E,E∖↑N}=∗ ▷P ∗ (▷P ={E∖↑N,E}=∗ q.[κ]).
   Proof.
     iIntros (??) "#LFT #HP Hκ". iDestruct "HP" as (i) "#[Hidx [[% Hinv]|[% Hinv]]]".
     - iInv N as ">Hi" "Hclose".
       iMod (idx_bor_acc with "LFT Hidx Hi Hκ") as "[$ Hclose']". solve_ndisj.
       iIntros "!> H". iMod ("Hclose'" with "H") as "[? $]". by iApply "Hclose".
-    - iMod (shr_bor_acc with "LFT []") as "[[$ Hclose]|[H† _]]"; try done.
+    - iMod (at_bor_acc with "LFT []") as "[[$ Hclose]|[H† _]]"; try done.
       + iExists i. auto.
       + subst. rewrite difference_twice_L. iIntros "!>HP". by iMod ("Hclose" with "HP").
       + iDestruct (lft_tok_dead with "Hκ H†") as "[]".
   Qed.
 
-  Lemma shr_bor_shorten κ κ': κ ⊑ κ' -∗ &shr{κ',N}P -∗ &shr{κ,N}P.
+  Lemma at_bor_shorten κ κ': κ ⊑ κ' -∗ &at{κ',N}P -∗ &at{κ,N}P.
   Proof.
     iIntros "#H⊑ H". iDestruct "H" as (i) "[??]". iExists i. iFrame.
       by iApply (idx_bor_shorten with "H⊑").
   Qed.
 
-  Lemma shr_bor_fake E κ:
-    ↑lftN ⊆ E → N ⊥ lftN → lft_ctx -∗ [†κ] ={E}=∗ &shr{κ,N}P.
+  Lemma at_bor_fake E κ:
+    ↑lftN ⊆ E → N ⊥ lftN → lft_ctx -∗ [†κ] ={E}=∗ &at{κ,N}P.
   Proof.
     iIntros (??) "#LFT#H†". iApply (bor_share with "[>]"); try done.
     by iApply (bor_fake with "LFT H†").
   Qed.
 
-  Lemma shr_bor_fake_lftN E κ:
-    ↑lftN ⊆ E → lft_ctx -∗ [†κ] ={E}=∗ &shr{κ,lftN}P.
+  Lemma at_bor_fake_lftN E κ:
+    ↑lftN ⊆ E → lft_ctx -∗ [†κ] ={E}=∗ &at{κ,lftN}P.
   Proof.
     iIntros (?) "#LFT#H†". iApply (bor_share_lftN with "[>]"); try done.
     by iApply (bor_fake with "LFT H†").
   Qed.
-End shared_bors.
+End atomic_bors.
 
-Lemma shr_bor_acc_lftN `{invG Σ, lftG Σ} (P : iProp Σ) E κ :
+Lemma at_bor_acc_lftN `{invG Σ, lftG Σ} (P : iProp Σ) E κ :
   ↑lftN ⊆ E →
-  lft_ctx -∗ &shr{κ,lftN}P ={E,E∖↑lftN}=∗ ▷P ∗ (▷P ={E∖↑lftN,E}=∗ True) ∨
+  lft_ctx -∗ &at{κ,lftN}P ={E,E∖↑lftN}=∗ ▷P ∗ (▷P ={E∖↑lftN,E}=∗ True) ∨
              [†κ] ∗ |={E∖↑lftN,E}=> True.
-Proof. intros. by rewrite (shr_bor_acc _ lftN) // difference_twice_L. Qed.
+Proof. intros. by rewrite (at_bor_acc _ lftN) // difference_twice_L. Qed.
 
-Typeclasses Opaque shr_bor.
+Typeclasses Opaque at_bor.
